high/Zeta.High.Verifier.fsti
@@ -112,7 +112,7 @@ let addm (#aprm: app_params)
          (k: base_key)
          (k': base_key)
          (vs: vtls_t aprm {vs.valid}):
-    (vs':vtls_t aprm {vs'.tid = vs.tid /\ vs'.clock = vs.clock})
+     (vs':vtls_t aprm {vs'.tid = vs.tid /\ vs'.clock = vs.clock})
   = let st = vs.st in
     let open Zeta.BinTree in
     let open Zeta.Merkle in
