steel/Zeta.HashFunction.fst
@@ -1,0 +1,52 @@
+module Zeta.HashFunction
+
+open Zeta.Hash
+open Zeta.App
+open Zeta.Record
+module T = Zeta.Steel.FormatsManual
+
+module ZSH = Zeta.Steel.HashValue
+module KU = Zeta.Steel.KeyUtils
+
+let lower_desc_hash (dh:Zeta.Merkle.desc_hash_t)
+  : GTot T.descendent_hash
+  = let open Zeta.Merkle in
+    match dh with
+    | Empty -> T.Dh_vnone ()
+    | Desc k h b -> 
+      let k = KU.lower_base_key k in
+      let h = Zeta.Steel.BitUtils.u256_of_bitvec h in
+      let b = if b then T.Vtrue else T.Vfalse in
+      T.(Dh_vsome ({ dhd_key = k;
+                     dhd_h = h;
+                     evicted_to_blum = b }))
+  
+let lower_value (v:value Zeta.Steel.ApplicationTypes.aprm)
+  : GTot T.value
+  = match v with
+    | AppV Null -> T.DValue None
+    | AppV (DValue iv) -> T.DValue (Some iv)
+    | IntV smv -> T.MValue ({ l = lower_desc_hash smv.left;
+                             r = lower_desc_hash smv.right })
+
+let ghashfn (#aprm:app_params) (v:value aprm)
+  : GTot hash_value
+  = let b = FStar.StrongExcludedMiddle.strong_excluded_middle 
+               (aprm == Zeta.Steel.ApplicationTypes.aprm)
+    in
+    if b 
+    then (
+      let tv = lower_value v in
+      let h = ZSH.hashfn tv in
+      Zeta.Steel.BitUtils.bitvec_of_u256 h
+    )
+    else (
+      zero
+    )
+
+assume
+val hashfn' (#aprm:app_params) (v:value aprm)
+  : Tot (h:hash_value { h == ghashfn v })
+
+let hashfn v = hashfn' v
+
