steel/Zeta.Steel.RelHashFunction.fst
@@ -1,0 +1,41 @@
+module Zeta.Steel.RelHashFunction
+friend Zeta.HashFunction
+open Zeta.Steel.Rel
+
+open Zeta.Hash
+open Zeta.App
+open Zeta.Record
+module T = Zeta.Steel.FormatsManual
+
+module ZSH = Zeta.Steel.HashValue
+module KU = Zeta.Steel.KeyUtils
+module ZH = Zeta.HashFunction
+
+let related_desc_hash_inv (sdh:T.descendent_hash)
+                          (idh:Zeta.Merkle.desc_hash_t)
+  : Lemma 
+    (requires related_desc_hash sdh idh)
+    (ensures ZH.lower_desc_hash idh == sdh)
+  = match sdh, idh with
+    | T.Dh_vnone _, _ -> ()
+    | T.Dh_vsome sdh, Zeta.Merkle.Desc k h b ->
+      BitUtils.inverse h
+  
+let related_val_inv (sv:s_val) (iv:i_val)
+  : Lemma 
+    (requires related_val sv iv)
+    (ensures ZH.lower_value iv == sv)
+  = match sv, iv with
+    | T.DValue None, _ -> ()
+    | T.DValue (Some sdv), _ -> ()
+    | T.MValue mv, IntV smv ->
+      related_desc_hash_inv mv.l smv.left;
+      related_desc_hash_inv mv.r smv.right
+
+(* the hash of two related values is related *)
+let related_hashfn (sv: s_val) (iv: i_val)
+  : Lemma (requires (related_val sv iv))
+          (ensures (related_hash_value (s_hashfn sv) (i_hashfn iv)))
+  = assert (ZH.hashfn iv ==
+           Zeta.Steel.BitUtils.bitvec_of_u256 (s_hashfn (ZH.lower_value iv)));
+    related_val_inv sv iv
