steel/Zeta.Steel.RelHashFunction.fsti
@@ -1,0 +1,7 @@
+module Zeta.Steel.RelHashFunction
+open Zeta.Steel.Rel
+
+(* the hash of two related values is related *)
+val related_hashfn (sv: s_val) (iv: i_val)
+  : Lemma (requires (related_val sv iv))
+          (ensures (related_hash_value (s_hashfn sv) (i_hashfn iv)))
